Lemmas.thy
@@ -11,7 +11,11 @@ lemma fresh_subst_type: "\<lbrakk> atom a \<sharp> \<tau> ; a = b \<or> atom a \
   by (nominal_induct \<sigma> avoiding: a b \<tau> rule: \<tau>.strong_induct) auto
 lemma fresh_subst_term_type: "\<lbrakk> atom a \<sharp> \<tau> ; a = b \<or> atom a \<sharp> e \<rbrakk> \<Longrightarrow> atom a \<sharp> subst_term_type e \<tau> b"
   by (nominal_induct e avoiding: a b \<tau> rule: term.strong_induct) (auto simp: fresh_subst_type)
-lemmas fresh_subst = fresh_subst_term fresh_subst_term_tyvar fresh_subst_type fresh_subst_term_type
+lemma fresh_subst_context_var: "atom x \<sharp> \<Gamma> \<Longrightarrow> atom (x::var) \<sharp> subst_context \<Gamma> \<tau>' a"
+  by (induction \<Gamma> \<tau>' a rule: subst_context.induct) (auto simp: fresh_Cons)
+lemma fresh_subst_context_tyvar: "\<lbrakk> atom a \<sharp> \<tau>' ; a = b \<or> atom a \<sharp> \<Gamma> \<rbrakk> \<Longrightarrow> atom a \<sharp> subst_context \<Gamma> \<tau>' b"
+  by (induction \<Gamma> \<tau>' a rule: subst_context.induct) (auto simp: fresh_Cons fresh_Nil fresh_subst_type)
+lemmas fresh_subst = fresh_subst_term fresh_subst_term_tyvar fresh_subst_type fresh_subst_term_type fresh_subst_context_var fresh_subst_context_tyvar
 
 (* atom c \<sharp> t \<Longrightarrow> t[t'/x] = ((x \<leftrightarrow> c) \<bullet> t)[t'/c] *)
 lemma subst_term_var_name: "atom c \<sharp> e \<Longrightarrow> subst_term e e' x = subst_term ((x \<leftrightarrow> c) \<bullet> e) e' c"
@@ -19,7 +23,7 @@ proof (nominal_induct e avoiding: c x e' rule: term.strong_induct)
   case (Let y \<tau> e1 e2)
   then have "(Let y \<tau> e1 e2)[e'/x] = Let y \<tau> e1[e'/x] e2[e'/x]" by auto
   also have "... = Let y \<tau> ((x \<leftrightarrow> c) \<bullet> e1)[e'/c] ((x \<leftrightarrow> c) \<bullet> e2)[e'/c]"
-    by (metis Let.hyps(1) Let.hyps(4) Let.hyps(5) Let.prems fresh_at_base(2) list.set(1) list.set(2) singletonD term.fresh(7)) sorry
+    by (metis Let.hyps(1) Let.hyps(4) Let.hyps(5) Let.prems fresh_at_base(2) list.set(1) list.set(2) singletonD term.fresh(7))
   also have "... = (Let y \<tau> ((x \<leftrightarrow> c) \<bullet> e1) ((x \<leftrightarrow> c) \<bullet> e2))[e'/c]" by (simp add: Let.hyps(1) Let.hyps(3))
   finally show ?case
     by (metis Let.hyps(1) Let.hyps(2) flip_fresh_fresh fresh_at_base(2) no_vars_in_ty term.perm_simps(7))
@@ -28,10 +32,10 @@ qed (auto simp: flip_fresh_fresh fresh_at_base)
 lemma subst_type_var_name: "atom c \<sharp> \<sigma> \<Longrightarrow> subst_type \<sigma> \<tau> a = subst_type ((a \<leftrightarrow> c) \<bullet> \<sigma>) \<tau> c"
 proof (nominal_induct \<sigma> avoiding: c a \<tau> rule: \<tau>.strong_induct)
   case (TyForall b k \<sigma>)
-  then have 1: "atom c \<sharp> \<sigma>" by (simp add: fresh_at_base)
-  have "subst_type \<sigma> \<tau> a = subst_type ((a \<leftrightarrow> c) \<bullet> \<sigma>) \<tau> c" by (rule TyForall(4)[OF 1])
-  then show ?case
-    by (smt TyForall.hyps(1) TyForall.hyps(2) TyForall.hyps(3) \<tau>.perm_simps(5) flip_fresh_fresh fresh_Pair fresh_at_base(2) no_tyvars_in_kinds subst_type.simps(5))
+  then have "(\<forall> b:k. \<sigma>)[\<tau>/a] = (\<forall> b:k. \<sigma>[\<tau>/a])" by simp
+  also have "... = (\<forall> b:k. ((a \<leftrightarrow> c) \<bullet> \<sigma>)[\<tau>/c])" by (metis TyForall.hyps(1) TyForall.hyps(4) TyForall.prems \<tau>.fresh(5) fresh_at_base(2) list.set(1) list.set(2) singletonD)
+  also have "... = (\<forall> b:k. ((a \<leftrightarrow> c) \<bullet> \<sigma>))[\<tau>/c]" by (simp add: TyForall.hyps(1) TyForall.hyps(3))
+  finally show ?case by (metis TyForall.hyps(1) TyForall.hyps(2) \<tau>.perm_simps(5) flip_fresh_fresh fresh_at_base(2) no_tyvars_in_kinds)
 qed (auto simp: fresh_at_base)
 
 lemma subst_term_type_var_name: "atom c \<sharp> e \<Longrightarrow> subst_term_type e \<tau> a = subst_term_type ((a \<leftrightarrow> c) \<bullet> e) \<tau> c"
@@ -52,6 +56,24 @@ next
   finally show ?case by (simp add: flip_fresh_fresh)
 qed (auto simp: flip_fresh_fresh fresh_at_base subst_type_var_name)
 lemmas subst_var_name = subst_term_var_name subst_type_var_name subst_term_type_var_name
+
+lemma subst_context_var_name: "atom c \<sharp> \<Gamma> \<Longrightarrow> subst_context \<Gamma> \<tau> a = subst_context ((a \<leftrightarrow> c) \<bullet> \<Gamma>) \<tau> c"
+proof (induction \<Gamma> \<tau> a rule: subst_context.induct)
+  case (3 b k \<Gamma> \<tau>' a)
+  then have 1: "\<Gamma>[\<tau>'/a] = ((a \<leftrightarrow> c) \<bullet> \<Gamma>)[\<tau>'/c]" by (auto simp: fresh_Cons)
+  have 2: "b \<noteq> c" using 3 binder.fresh(2) fresh_Cons fresh_at_base(2) by blast 
+  then show ?case
+  proof (cases "a = b")
+    case True
+    then show ?thesis using 1 by auto
+  next
+    case False
+    then have a: "(BTyVar b k # \<Gamma>)[\<tau>'/a] = BTyVar b k # \<Gamma>[\<tau>'/a]" by simp
+    from False have b: "((a \<leftrightarrow> c) \<bullet> (BTyVar b k # \<Gamma>))[\<tau>'/c] = ((a \<leftrightarrow> c) \<bullet> BTyVar b k) # ((a \<leftrightarrow> c) \<bullet> \<Gamma>)[\<tau>'/c]" using flip_fresh_fresh 2 by simp
+    have c: "(a \<leftrightarrow> c) \<bullet> BTyVar b k = BTyVar b k" using False 2 flip_fresh_fresh by force
+    show ?thesis using a b c 1 by argo
+  qed
+qed (auto simp: flip_fresh_fresh fresh_Cons subst_type_var_name)
 
 (* [[atom a]]lst. t = [[atom a2]]lst. t2 \<Longrightarrow> subst t t' a = subst t2 t' a2 *)
 lemma subst_term_same: "[[atom a]]lst. e = [[atom a']]lst. e' \<Longrightarrow> subst_term e t a = subst_term e' t a'"
@@ -91,16 +113,22 @@ proof (induction e \<tau> a rule: subst_term_type.induct)
   case (6 b \<tau> a k e2)
   then show ?case by (simp add: "6.hyps" fresh_Pair fresh_at_base(2))
 qed (auto simp: fresh_subst_type_same)
-lemmas fresh_subst_same = fresh_subst_term_same fresh_subst_type_same fresh_subst_term_type_same
 
-(* \<lbrakk> x \<noteq> y ; atom x \<sharp> t1 \<rbrakk> \<Longrightarrow> subst (subst x t2 e) t1 y = subst (subst e t1 y) (subst t2 t1 y) x *)
+lemma fresh_subst_context_same: "atom a \<sharp> \<Gamma> \<Longrightarrow> subst_context \<Gamma> \<tau> a = \<Gamma>"
+  by (induction \<Gamma> \<tau> a rule: subst_context.induct) (auto simp: fresh_Cons fresh_subst_type_same)
+
+lemmas fresh_subst_same = fresh_subst_term_same fresh_subst_type_same fresh_subst_term_type_same fresh_subst_context_same
+
+(* \<lbrakk> x \<noteq> y ; atom x \<sharp> t1 \<rbrakk> \<Longrightarrow> subst (subst e t2 x) t1 y = subst (subst e t1 y) (subst t2 t1 y) x *)
 lemma subst_subst_term: "\<lbrakk> x \<noteq> y ; atom x \<sharp> t1 \<rbrakk> \<Longrightarrow> subst_term (subst_term e t2 x) t1 y = subst_term (subst_term e t1 y) (subst_term t2 t1 y) x"
   by (nominal_induct e avoiding: x y t1 t2 rule: term.strong_induct) (auto simp: fresh_subst_same fresh_subst)
 lemma subst_subst_type: "\<lbrakk> a \<noteq> b ; atom a \<sharp> \<tau>1 \<rbrakk> \<Longrightarrow> subst_type (subst_type \<sigma> \<tau>2 a) \<tau>1 b = subst_type (subst_type \<sigma> \<tau>1 b) (subst_type \<tau>2 \<tau>1 b) a"
   by (nominal_induct \<sigma> avoiding: a b \<tau>1 \<tau>2 rule: \<tau>.strong_induct) (auto simp: fresh_subst_same fresh_subst)
 lemma subst_subst_term_type: "\<lbrakk> a \<noteq> b ; atom a \<sharp> \<tau>1 \<rbrakk> \<Longrightarrow> subst_term_type (subst_term_type e \<tau>2 a) \<tau>1 b = subst_term_type (subst_term_type e \<tau>1 b) (subst_type \<tau>2 \<tau>1 b) a"
   by (nominal_induct e avoiding: a b \<tau>1 \<tau>2 rule: term.strong_induct) (auto simp: fresh_subst_same fresh_subst subst_subst_type)
-lemmas subst_subst = subst_subst_term subst_subst_type subst_subst_term_type
+lemma subst_subst_context: "\<lbrakk> a \<noteq> b; atom a \<sharp> \<tau>1 \<rbrakk> \<Longrightarrow> subst_context (subst_context \<Gamma> \<tau>2 a) \<tau>1 b = subst_context (subst_context \<Gamma> \<tau>1 b) (subst_type \<tau>2 \<tau>1 b) a"
+  by (induction \<Gamma> \<tau>2 a rule: subst_context.induct) (auto simp: subst_subst_type)
+lemmas subst_subst = subst_subst_term subst_subst_type subst_subst_term_type subst_subst_context
 
 (* misc *)
 lemma fv_supp_subset: "fv_\<tau> \<tau> \<subseteq> supp \<tau>"
