Soundness.thy
@@ -3,15 +3,16 @@ theory Soundness
 begin
 
 no_notation Set.member ("(_/ \<in> _)" [51, 51] 50)
+no_notation Set.member  ("(_/ : _)" [51, 51] 50)
 
 declare term.fv_defs[simp]
 declare \<tau>.fv_defs[simp]
 
 theorem progress: "[] \<turnstile> e : \<tau> \<Longrightarrow> is_value e \<or> (\<exists>e'. e \<longrightarrow> e')"
-proof (induction "[] :: \<Gamma>" e \<tau> rule: T.induct)
-case (T_AppI e1 \<tau>1 \<tau>2 e2)
-  note IH1 = T_AppI(2)
-  note IH2 = T_AppI(4)
+proof (induction "[] :: \<Gamma>" e \<tau> rule: Tm_induct)
+case (App e1 e2 \<tau>1 \<tau>2)
+  note IH1 = App(2)
+  note IH2 = App(4)
 
   from IH1 show ?case
   proof (elim disjE)
@@ -19,12 +20,12 @@ case (T_AppI e1 \<tau>1 \<tau>2 e2)
     from IH2 show ?thesis
     proof (elim disjE)
       assume "is_value e2"
-      from \<open>is_value e1\<close> T_AppI(1) have "\<exists>x e. e1 = (\<lambda>x:\<tau>1. e)" by (simp add: fun_ty_lam)
+      from \<open>is_value e1\<close> App(1) have "\<exists>x e. e1 = (\<lambda>x:\<tau>1. e)" by (simp add: fun_ty_lam)
       then have "\<exists>e'. Step (App e1 e2) e'" using \<open>is_value e2\<close> ST_BetaI by blast
       then show ?thesis by simp
     next
       assume "\<exists>e2'. Step e2 e2'"
-      then show ?thesis using ST_BetaI T_AppI.hyps(1) \<open>is_value e1\<close> fun_ty_lam by blast
+      then show ?thesis using ST_BetaI App.hyps(1) \<open>is_value e1\<close> fun_ty_lam by blast
     qed
   next
     assume "\<exists>e1'. Step e1 e1'"
@@ -33,338 +34,164 @@ case (T_AppI e1 \<tau>1 \<tau>2 e2)
     then show ?thesis by blast
   qed
 next
-  case (T_LetI x e1 \<tau>1 e2 \<tau>2)
+  case (Let e1 e2 \<tau>1 \<tau>2 x)
   then show ?case using ST_SubstI by blast
 next
-  case (T_AppTI e a \<sigma> \<tau>)
-  from T_AppTI(2) show ?case
+  case (TApp a k e \<sigma> \<tau>)
+  from TApp(2) show ?case
   proof (elim disjE)
     assume "is_value e"
-    then obtain b k e1 where "e = (\<Lambda> b : k . e1)" using T_AppTI
-      by (smt T.simps \<tau>.distinct(17) \<tau>.distinct(7) is_value.simps(1) is_value.simps(4) is_value.simps(5) is_value.simps(7))
-    then show ?thesis using Step.ST_BetaTI T_AppTI by blast
+    then obtain b k e1 where "e = (\<Lambda> b : k . e1)" using TApp.hyps(1) forall_ty_lam by blast
+    then show ?thesis using Step.ST_BetaTI TApp by blast
   next
     assume "\<exists>e'. Step e e'"
     then show ?thesis using ST_AppTI by fast
   qed
 qed auto
 
-lemma context_invariance_ty:
-  assumes "\<Gamma> \<turnstile>\<^sub>t\<^sub>y \<tau> : k"
-  and has_tyvars: "\<forall>a k. Set.member (atom a) (fv_\<tau> \<tau>) \<and> BTyVar a k \<in> \<Gamma> \<longrightarrow> BTyVar a k \<in> \<Gamma>'"
-  shows "\<Gamma>' \<turnstile>\<^sub>t\<^sub>y \<tau> : k"
-using assms proof (nominal_induct \<Gamma> \<tau> k avoiding: \<Gamma>' rule: Ty.strong_induct)
-  case (Ty_Var a \<Gamma>)
-  then show ?case using supp_at_base Ty.Ty_Var by fastforce
+lemma weaken_isin: "\<lbrakk> bndr \<in> (\<Gamma> @ \<Gamma>') ; \<turnstile> \<Gamma> @ xs @ \<Gamma>' \<rbrakk> \<Longrightarrow> bndr \<in> (\<Gamma> @ xs @ \<Gamma>')"
+proof (induction \<Gamma> arbitrary: bndr \<Gamma>' xs)
+  case Nil
+  then show ?case by (cases bndr rule: binder.exhaust) (auto simp: isin_subset)
 next
-  case (Ty_App \<Gamma> \<tau>1 \<kappa>1 \<kappa>2 \<tau>2)
-  then show ?case by (metis Ty.Ty_App UnCI \<tau>.fv_defs(4))
-qed (auto intro: Ty.intros)
-
-lemma context_invariance:
-  assumes "\<Gamma> \<turnstile> e : \<tau>"
-  and has_vars: "\<forall>x \<tau>'. Set.member (atom x) (fv_term e) \<and> BVar x \<tau>' \<in> \<Gamma> \<longrightarrow> BVar x \<tau>' \<in> \<Gamma>'"
-  and has_tyvars: "\<forall>a k. Set.member (atom a) (fv_term e) \<and> BTyVar a k \<in> \<Gamma> \<longrightarrow> BTyVar a k \<in> \<Gamma>'"
-  shows "\<Gamma>' \<turnstile> e : \<tau>"
-using assms proof (nominal_induct \<Gamma> e \<tau> avoiding: \<Gamma>' rule: T.strong_induct)
-  case (T_AbsI x \<Gamma> \<tau>1 e \<tau>2)
-  then have 1: "BVar x \<tau>1 # \<Gamma>' \<turnstile> e : \<tau>2" by auto
-  have 2: "\<Gamma>' \<turnstile>\<^sub>t\<^sub>y \<tau>1 : \<star>" using context_invariance_ty[OF T_AbsI(3)] T_AbsI(7) fv_supp_subset by (simp add: subset_eq)
-  show ?case by (rule T.T_AbsI[OF T_AbsI(1) 2 1])
-next
-  case (T_AppI \<Gamma> e1 \<tau>1 \<tau>2 e2)
-  then show ?case by (metis T.T_AppI Un_iff term.fv_defs(2))
-next
-  case (T_LetI x \<Gamma> e1 \<tau>1 e2 \<tau>2)
-  then have 1: "BVar x \<tau>1 # \<Gamma>' \<turnstile> e2 : \<tau>2" by auto
-  from T_LetI have 2: "atom x \<sharp> (\<Gamma>', e1)" by auto
-  from T_LetI have 3: "\<Gamma>' \<turnstile> e1 : \<tau>1" by force
-  show ?case by (rule T.T_LetI[OF 2 1 3])
-next
-  case (T_AppTI \<Gamma> e a k \<sigma> \<tau>)
-  then have 1: "\<Gamma>' \<turnstile> e : \<forall> a : k . \<sigma>" by simp
-  have 2: "\<Gamma>' \<turnstile>\<^sub>t\<^sub>y \<tau> : k" using context_invariance_ty[OF T_AppTI(3)] T_AppTI(5) fv_supp_subset by (simp add: subset_eq)
-  show ?case by (rule T.T_AppTI[OF 1 2])
-next
-  case (T_AbsTI a k \<Gamma> e \<sigma>)
-  then have 1: "BTyVar a k # \<Gamma>' \<turnstile> e : \<sigma>" by auto
-  have 2: "atom a \<sharp> \<Gamma>'" using T_AbsTI by auto
-  show ?case by (rule T.T_AbsTI[OF 1 2])
-qed (auto intro: T.intros simp: supp_at_base)
-
-lemma substitution: "\<lbrakk> BVar x \<tau>'#\<Gamma> \<turnstile> e : \<tau> ; [] \<turnstile> v : \<tau>' \<rbrakk> \<Longrightarrow> \<Gamma> \<turnstile> subst_term v x e : \<tau>"
-proof (nominal_induct e avoiding: \<Gamma> \<tau> v x \<tau>' rule: term.strong_induct)
-  case (Var y)
+  case (Cons b \<Gamma>)
+  have 1: "\<turnstile> \<Gamma> @ xs @ \<Gamma>'" using Cons(3) Ctx.cases by auto
   then show ?case
-  proof (cases "y = x")
-    case True
-    then have "\<tau> = \<tau>'" using T.cases Var(1) by fastforce
-    then show ?thesis using True Var(2) context_invariance by fastforce
+  proof (cases b rule: binder.exhaust)
+    case (BVar x \<tau>)
+    then show ?thesis using 1 Cons by (cases bndr rule: binder.exhaust) auto
   next
-    case False
-    have "fv_term (Var y) = {atom y}" using supp_at_base by auto
-    then have "\<Gamma> \<turnstile> Var y : \<tau>" using context_invariance[OF Var(1)] False by auto
-    then show ?thesis using False by simp
+    case (BTyVar a k)
+    then show ?thesis using 1 Cons by (cases bndr rule: binder.exhaust) auto
   qed
-next
-  case (App e1 e2)
-  obtain \<tau>1 where 1: "BVar x \<tau>' # \<Gamma> \<turnstile> e1 : (\<tau>1 \<rightarrow> \<tau>)" "BVar x \<tau>' # \<Gamma> \<turnstile> e2 : \<tau>1" by (cases rule: T.cases[OF App(3)]) auto
-  have 2: "\<Gamma> \<turnstile> subst_term v x e1 : (\<tau>1 \<rightarrow> \<tau>)" by (rule App(1)[OF 1(1) App(4)])
-  have 3: "\<Gamma> \<turnstile> subst_term v x e2 : \<tau>1" by (rule App(2)[OF 1(2) App(4)])
-  show ?case using T.T_AppI[OF 2 3] by simp
-next
-  case (TyApp e1 \<sigma>)
-  then show ?case
-    by (smt T.cases T_AppTI context_invariance_ty isin.simps(4) subst_term.simps(5) term.distinct(13) term.distinct(23) term.distinct(25) term.distinct(27) term.distinct(29) term.distinct(3) term.eq_iff(3))
-next
-  case Unit
-  have "\<tau> = TyUnit" by (cases rule: T.cases[OF Unit(1)]) auto
-  then show ?case using T.T_UnitI by simp
-next
-  case (Lam y \<sigma> e')
-  then have 1: "atom y \<sharp> BVar x \<tau>' # \<Gamma>" by (simp add: fresh_Cons)
-  obtain \<tau>2 where P: "BVar y \<sigma> # BVar x \<tau>' # \<Gamma> \<turnstile> e' : \<tau>2" "\<tau> = (\<sigma> \<rightarrow> \<tau>2)" "BVar x \<tau>' # \<Gamma> \<turnstile>\<^sub>t\<^sub>y \<sigma> : \<star>" using T_Abs_Inv[OF Lam(7) 1] by blast
-  then have 2: "BVar x \<tau>' # BVar y \<sigma> # \<Gamma> \<turnstile> e' : \<tau>2" using Lam(4) context_invariance by auto
-  from P have 3: "\<Gamma> \<turnstile>\<^sub>t\<^sub>y \<sigma> : \<star>" using context_invariance_ty by auto
-  from Lam show ?case using T.T_AbsI[OF Lam(1) 3] P 2 by auto
-next
-  case (TyLam a k e)
-  have 1: "atom a \<sharp> BVar x \<tau>' # \<Gamma>" by (simp add: TyLam.hyps(1) TyLam.hyps(5) fresh_Cons)
-  obtain \<sigma> where P: "BTyVar a k # BVar x \<tau>' # \<Gamma> \<turnstile> e : \<sigma>" "\<tau> = (\<forall> a : k . \<sigma>)" using T_AbsT_Inv[OF TyLam(7) 1 TyLam(2)] by blast
-  then have 1: "BVar x \<tau>' # BTyVar a k # \<Gamma> \<turnstile> e : \<sigma>" using context_invariance by fastforce
-  have 2: "BTyVar a k # \<Gamma> \<turnstile> subst_term v x e : \<sigma>" by (rule TyLam(6)[OF 1 TyLam(8)])
-  from TyLam show ?case using T.T_AbsTI[OF 2 TyLam(1)] P by auto
-next
-  case (Let y \<tau>1 e1 e2)
-  then have 1: "atom y \<sharp> BVar x \<tau>' # \<Gamma>" by (simp add: fresh_Cons)
-  have P: "BVar x \<tau>' # \<Gamma> \<turnstile> e1 : \<tau>1" "BVar y \<tau>1 # BVar x \<tau>' # \<Gamma> \<turnstile> e2 : \<tau>" using T_Let_Inv[OF Let(8) 1] by auto
-  have 2: "\<Gamma> \<turnstile> subst_term v x e1 : \<tau>1" by (rule Let(6)[OF P(1) Let(9)])
-  have 3: "BVar x \<tau>' # BVar y \<tau>1 # \<Gamma> \<turnstile> e2 : \<tau>" using Let(4) P(2) context_invariance by auto
-  have 4: "BVar y \<tau>1 # \<Gamma> \<turnstile> subst_term v x e2 : \<tau>" by (rule Let(7)[OF 3 Let(9)])
-  have "atom y \<sharp> subst_term v x e1" using "2" Let(1) fresh_term_var by blast
-  then have 6: "atom y \<sharp> (\<Gamma>, subst_term v x e1)" using Let(1) by auto
-  show ?case using T.T_LetI[OF 6 4 2] Let by auto
 qed
 
-lemma type_substitution_ty: "\<lbrakk> BTyVar a k # \<Gamma> \<turnstile>\<^sub>t\<^sub>y \<tau> : k2 ; \<Gamma> \<turnstile>\<^sub>t\<^sub>y \<tau>' : k ; atom a \<sharp> \<Gamma> \<rbrakk> \<Longrightarrow> \<Gamma> \<turnstile>\<^sub>t\<^sub>y subst_type \<tau>' a \<tau> : k2"
-proof (nominal_induct \<tau> avoiding: a \<Gamma> \<tau>' k k2 rule: \<tau>.strong_induct)
- case TyUnit
-  then show ?case using context_invariance_ty by auto
+lemma weaken_ty: "\<lbrakk> \<Gamma> @ \<Gamma>' \<turnstile>\<^sub>t\<^sub>y \<tau> : k ; \<turnstile> \<Gamma> @ xs @ \<Gamma>' \<rbrakk> \<Longrightarrow> \<Gamma> @ xs @ \<Gamma>' \<turnstile>\<^sub>t\<^sub>y \<tau> : k"
+proof (nominal_induct \<tau> avoiding: \<Gamma> \<Gamma>' xs k rule: \<tau>.strong_induct)
+  case TyUnit
+  then have "k = \<star>" by (cases rule: Ty.cases[OF TyUnit(1)]) auto
+  then show ?case using Ty_Unit[OF TyUnit(2)] by simp
 next
   case (TyVar x)
-  then show ?case
-  proof (cases "atom x = atom a")
-    case True
-    then have "k = k2" using Ty.cases TyVar.prems(1) by force
-    then show ?thesis using TyVar True by auto
-  next
-    case False
-    then show ?thesis
-      by (smt TyVar.prems(1) TyVar.prems(2) TyVar.prems(3) \<tau>.fv_defs(2) \<tau>.supp(2) context_invariance_ty fresh_def fresh_subst_type isin.simps(5) subst_type.simps(2) ty_fresh_vars)
-  qed
+  have 1: "BTyVar x k \<in> (\<Gamma> @ \<Gamma>')" by (cases rule: Ty.cases[OF TyVar(1)]) auto
+  show ?case by (rule Ty_Var[OF TyVar(2) weaken_isin[OF 1 TyVar(2)]])
 next
-  case (TyArrow e1 e2)
-  then have 1: "k2 = \<star>" using Ty.cases[OF TyArrow(3)] by (smt \<tau>.distinct(15) \<tau>.distinct(9))
-  then have "BTyVar a k # \<Gamma> \<turnstile>\<^sub>t\<^sub>y e1 : \<star>" "BTyVar a k # \<Gamma> \<turnstile>\<^sub>t\<^sub>y e2 : \<star>" using Ty.cases[OF TyArrow(3)] by auto
-  then show ?case using TyArrow 1 Ty_Arrow by auto
+  case (TyArrow \<tau>1 \<tau>2)
+  have "k = \<star> \<and> \<Gamma> @ \<Gamma>' \<turnstile>\<^sub>t\<^sub>y \<tau>1 : \<star> \<and> \<Gamma> @ \<Gamma>' \<turnstile>\<^sub>t\<^sub>y \<tau>2 : \<star>" by (cases rule: Ty.cases[OF TyArrow(3)]) auto
+  then have 1: "k = \<star>" "\<Gamma> @ \<Gamma>' \<turnstile>\<^sub>t\<^sub>y \<tau>1 : \<star>" "\<Gamma> @ \<Gamma>' \<turnstile>\<^sub>t\<^sub>y \<tau>2 : \<star>" by auto
+  have 2: "\<Gamma> @ xs @ \<Gamma>' \<turnstile>\<^sub>t\<^sub>y \<tau>1 : \<star>" by (rule TyArrow(1)[OF 1(2) TyArrow(4)])
+  have 3: "\<Gamma> @ xs @ \<Gamma>' \<turnstile>\<^sub>t\<^sub>y \<tau>2 : \<star>" by (rule TyArrow(2)[OF 1(3) TyArrow(4)])
+  show ?case using Ty_FunArrow[OF 2 3] 1(1) by simp
 next
   case (TyConApp \<tau>1 \<tau>2)
-  then obtain k1 where "BTyVar a k # \<Gamma> \<turnstile>\<^sub>t\<^sub>y \<tau>1 : KArrow k1 k2 \<and> BTyVar a k # \<Gamma> \<turnstile>\<^sub>t\<^sub>y \<tau>2 : k1" using Ty.cases[OF TyConApp(3)] by fastforce
-  then show ?case using TyConApp Ty_App by fastforce
+  obtain k1 where P: "\<Gamma> @ \<Gamma>' \<turnstile>\<^sub>t\<^sub>y \<tau>1 : KArrow k1 k" "\<Gamma> @ \<Gamma>' \<turnstile>\<^sub>t\<^sub>y \<tau>2 : k1" by (cases rule: Ty.cases[OF TyConApp(3)]) auto
+  have 2: "\<Gamma> @ xs @ \<Gamma>' \<turnstile>\<^sub>t\<^sub>y \<tau>1 : KArrow k1 k" by (rule TyConApp(1)[OF P(1) TyConApp(4)])
+  have 3: "\<Gamma> @ xs @ \<Gamma>' \<turnstile>\<^sub>t\<^sub>y \<tau>2 : k1" by (rule TyConApp(2)[OF P(2) TyConApp(4)])
+  show ?case by (rule Ty_App[OF 2 3])
 next
-  case (TyForall b k3 \<tau>)
-  then have "k2 = \<star>" using Ty.cases by fastforce
-  have "BTyVar b k3 # BTyVar a k # \<Gamma> \<turnstile>\<^sub>t\<^sub>y \<tau> : \<star>" proof (cases rule: Ty.cases[OF TyForall(7)])
-    case (5 c k4 \<Gamma>2 \<sigma>)
-    then have 1: "\<tau> = (b \<leftrightarrow> c) \<bullet> \<sigma>" by (smt Abs1_eq_iff(3) TyForall.prems(1) \<tau>.eq_iff(5) \<tau>.perm_simps(5) flip_at_simps(2) flip_def swap_fresh_fresh ty_fresh_vars)
-    from 5 have "k4 = k3" by auto
-    then have "(b \<leftrightarrow> c) \<bullet> (BTyVar c k3 # \<Gamma>2 \<turnstile>\<^sub>t\<^sub>y \<sigma> : \<star>)" using 5(4) by simp
-    then have 2: "((b \<leftrightarrow> c) \<bullet> BTyVar c k3) # \<Gamma>2 \<turnstile>\<^sub>t\<^sub>y (b \<leftrightarrow> c) \<bullet> \<sigma> : \<star>" by (smt "5"(1) "5"(4) "5"(5) Cons_eqvt Ty.eqvt TyForall.hyps(1) TyForall.hyps(2) TyForall.hyps(4) \<kappa>.perm_simps(1) \<open>k4 = k3\<close> binder.fresh(2) flip_def fresh_Cons swap_fresh_fresh)
-    have "(b \<leftrightarrow> c) \<bullet> BTyVar c k3 = BTyVar b k3" by (simp add: flip_def swap_fresh_fresh)
-    then show ?thesis using 1 2 5(1) by argo
-  qed auto
-  then have 1: "BTyVar a k # BTyVar b k3 # \<Gamma> \<turnstile>\<^sub>t\<^sub>y \<tau> : \<star>" using context_invariance_ty TyForall(1) by auto
-  have 2: "BTyVar b k3 # \<Gamma> \<turnstile>\<^sub>t\<^sub>y \<tau>' : k" using context_invariance_ty[OF TyForall(8)] by (simp add: TyForall.hyps(2) fresh_not_isin_tyvar)
-  have 3: "BTyVar b k3 # \<Gamma> \<turnstile>\<^sub>t\<^sub>y subst_type \<tau>' a \<tau> : \<star>" using TyForall(6)[OF 1 2] using TyForall.hyps(1) TyForall.prems(3) fresh_Cons by fastforce
-  then show ?case by (simp add: TyForall.hyps(1) TyForall.hyps(2) TyForall.hyps(3) Ty_Forall \<open>k2 = \<star>\<close>)
+  case (TyForall a k1 \<sigma>)
+  have P: "(BTyVar a k1 # \<Gamma>) @ \<Gamma>' \<turnstile>\<^sub>t\<^sub>y \<sigma> : \<star>" "k = \<star>" using Ty_Forall_Inv[OF TyForall(6)] TyForall(1,2) fresh_append by auto
+  have 1: "atom a \<sharp> \<Gamma> @ xs @ \<Gamma>'" using TyForall(1-3) fresh_append by blast
+  have 2: "\<turnstile> (BTyVar a k1 # \<Gamma>) @ xs @ \<Gamma>'" using Ctx_TyVar[OF TyForall(7) 1] by simp
+  have 3: "BTyVar a k1 # \<Gamma> @ xs @ \<Gamma>' \<turnstile>\<^sub>t\<^sub>y \<sigma> : \<star>" using TyForall(5)[OF P(1) 2] by simp
+  show ?case using Ty_Forall[OF 3] P(2) by simp
 qed
 
-lemma type_substitution:
-  assumes well_typed: "BTyVar a k # \<Gamma> \<turnstile> e : \<sigma>" "\<Gamma> \<turnstile>\<^sub>t\<^sub>y \<tau>' : k"
-  and context_tyvar: "\<forall>b k. BTyVar b k \<in> \<Gamma> \<longrightarrow> BTyVar b k \<in> \<Gamma>'"
-  and context_var: "\<forall>x \<tau>. BVar x \<tau> \<in> \<Gamma> \<longrightarrow> BVar x (subst_type \<tau>' a \<tau>) \<in> \<Gamma>'"
-  and fresh: "atom a \<sharp> \<Gamma>'"
-shows "\<Gamma>' \<turnstile> subst_term_type \<tau>' a e : subst_type \<tau>' a \<sigma>"
-using assms proof (nominal_induct e avoiding: a k \<Gamma> \<Gamma>' \<sigma> \<tau>' rule: term.strong_induct)
+lemma weaken_tm: "\<lbrakk> \<Gamma> @ \<Gamma>' \<turnstile> e : \<tau> ; \<turnstile> \<Gamma> @ xs @ \<Gamma>' \<rbrakk> \<Longrightarrow> \<Gamma> @ xs @ \<Gamma>' \<turnstile> e : \<tau>"
+proof (nominal_induct e avoiding: \<Gamma> \<Gamma>' xs \<tau> rule: term.strong_induct)
   case (Var x)
-  then have 1: "BVar x (subst_type \<tau>' a \<sigma>) \<in> \<Gamma>'"
-    by (smt T.cases isin.simps(3) term.distinct(1) term.distinct(11) term.distinct(3) term.distinct(5) term.distinct(7) term.distinct(9) term.eq_iff(1))
-  show ?case using T.T_VarI[OF 1] by simp
+  then have 1: "BVar x \<tau> \<in> (\<Gamma> @ \<Gamma>')" by (cases rule: Tm.cases[OF Var(1)]) auto
+  have 2: "BVar x \<tau> \<in> (\<Gamma> @ xs @ \<Gamma>')" by (rule weaken_isin[OF 1 Var(2)])
+  show ?case by (rule Tm_Var[OF Var(2) 2])
 next
   case (App e1 e2)
-  obtain \<tau>1 where "BTyVar a k # \<Gamma> \<turnstile> e1 : (\<tau>1 \<rightarrow> \<sigma>) \<and> BTyVar a k # \<Gamma> \<turnstile> e2 : \<tau>1" using T.cases[OF App(3)] by fastforce
-  then have P: "BTyVar a k # \<Gamma> \<turnstile> e1 : (\<tau>1 \<rightarrow> \<sigma>)" "BTyVar a k # \<Gamma> \<turnstile> e2 : \<tau>1" by auto
-
-  have 1: "\<Gamma>' \<turnstile> subst_term_type \<tau>' a e1 : subst_type \<tau>' a \<tau>1 \<rightarrow> subst_type \<tau>' a \<sigma>" using App(1)[OF P(1) App(4) App(5) App(6) App(7)] by simp
-  have 2: "\<Gamma>' \<turnstile> subst_term_type \<tau>' a e2 : subst_type \<tau>' a \<tau>1" by (rule App(2)[OF P(2) App(4) App(5) App(6) App(7)])
-
-  then show ?case using T.T_AppI[OF 1 2] by simp
+  obtain \<tau>1 where P: "\<Gamma> @ \<Gamma>' \<turnstile> e1 : \<tau>1 \<rightarrow> \<tau>" "\<Gamma> @ \<Gamma>' \<turnstile> e2 : \<tau>1" by (cases rule: Tm.cases[OF App(3)]) auto
+  have 1: "\<Gamma> @ xs @ \<Gamma>' \<turnstile> e1 : \<tau>1 \<rightarrow> \<tau>" by (rule App(1)[OF P(1) App(4)])
+  have 2: "\<Gamma> @ xs @ \<Gamma>' \<turnstile> e2 : \<tau>1" by (rule App(2)[OF P(2) App(4)])
+  show ?case by (rule Tm_App[OF 1 2])
 next
-  case (TyApp e \<tau>)
-
-  have "\<exists>b k2 \<sigma>'. BTyVar a k # \<Gamma> \<turnstile> e : (\<forall>b : k2 . \<sigma>') \<and> atom b \<sharp> a \<and> \<sigma> = subst_type \<tau> b \<sigma>' \<and> atom b \<sharp> \<tau>' \<and> BTyVar a k # \<Gamma> \<turnstile>\<^sub>t\<^sub>y \<tau> : k2"
-  proof (cases rule: T.cases[OF TyApp(2)])
-    case (6 \<Gamma>2 t b k2 \<sigma>2 \<tau>2)
-    then have 1: "BTyVar a k # \<Gamma> \<turnstile> e : \<forall> b : k2 . \<sigma>2" "\<sigma> = subst_type \<tau> b \<sigma>2" "BTyVar a k # \<Gamma> \<turnstile>\<^sub>t\<^sub>y \<tau> : k2" by auto
-    obtain c::tyvar where "atom c \<sharp> (a, b, \<sigma>2, \<tau>')" using obtain_fresh by blast
-    then have c: "atom c \<sharp> b" "atom c \<sharp> \<sigma>2" "atom c \<sharp> a" "atom c \<sharp> \<tau>'" using fresh_Pair by auto
-    from 1(1) have 2: "BTyVar a k # \<Gamma> \<turnstile> e : \<forall> c : k2 . (b \<leftrightarrow> c) \<bullet> \<sigma>2" by (smt Abs1_eq_iff(3) \<tau>.eq_iff(5) c(1) c(2) flip_commute fresh_at_base(2))
-    from 1(2) have "\<sigma> = subst_type \<tau> c ((b \<leftrightarrow> c) \<bullet> \<sigma>2)" using subst_type_var_name c by auto
-    then show ?thesis using 2 c(3) c(4) 1(3) by blast
-  qed auto
-  then obtain b k2 \<sigma>' where P: "BTyVar a k # \<Gamma> \<turnstile> e : (\<forall>b : k2 . \<sigma>')" "atom b \<sharp> a" "\<sigma> = subst_type \<tau> b \<sigma>'" "atom b \<sharp> \<tau>'" "BTyVar a k # \<Gamma> \<turnstile>\<^sub>t\<^sub>y \<tau> : k2" by blast
-
-  have 1: "\<Gamma>' \<turnstile>\<^sub>t\<^sub>y \<tau>' : k" using context_invariance_ty[OF TyApp(3)] using TyApp.prems(3) by blast
-  have 2: "BTyVar a k # \<Gamma>' \<turnstile>\<^sub>t\<^sub>y \<tau> : k2" using context_invariance_ty[OF P(5)] by (smt TyApp.prems(3) isin.simps(5))
-  have 3: "\<Gamma>' \<turnstile>\<^sub>t\<^sub>y subst_type \<tau>' a \<tau> : k2" by (rule type_substitution_ty[OF 2 1 TyApp(6)])
-  have 4: "\<Gamma>' \<turnstile> subst_term_type \<tau>' a e : \<forall> b : k2 . subst_type \<tau>' a \<sigma>'" using TyApp(1)[OF P(1) TyApp(3) TyApp(4) TyApp(5) TyApp(6)] P(2) P(4) by auto
-
-  have "\<Gamma>' \<turnstile> TyApp (subst_term_type \<tau>' a e) (subst_type \<tau>' a \<tau>) : subst_type \<tau>' a (subst_type \<tau> b \<sigma>')" using T.T_AppTI[OF 4 3] subst_type_order[OF P(4) P(2)] by simp
-  then show ?case using P(3) by simp
+  case (TyApp e \<sigma>)
+  obtain a k \<sigma>1 where P: "\<Gamma> @ \<Gamma>' \<turnstile> e : \<forall> a:k. \<sigma>1" "\<Gamma> @ \<Gamma>' \<turnstile>\<^sub>t\<^sub>y \<sigma> : k" "\<tau> = \<sigma>1[\<sigma>/a]" by (cases rule: Tm.cases[OF TyApp(2)]) auto
+  have 1: "\<Gamma> @ xs @ \<Gamma>' \<turnstile> e : \<forall> a:k. \<sigma>1" by (rule TyApp(1)[OF P(1) TyApp(3)])
+  have 2: "\<Gamma> @ xs @ \<Gamma>' \<turnstile>\<^sub>t\<^sub>y \<sigma> : k" by (rule weaken_ty[OF P(2) TyApp(3)])
+  show ?case using Tm_TApp[OF 1 2] P(3) by simp
 next
   case Unit
-  then have "\<sigma> = TyUnit" using T.cases by fastforce
-  then show ?case using T.T_UnitI by simp
+  then have "\<tau> = TyUnit" by (cases rule: Tm.cases[OF Unit(1)]) auto
+  then show ?case using Tm_Unit[OF Unit(2)] by simp
 next
   case (Lam x \<tau>1 e)
-  then have 1: "atom x \<sharp> BTyVar a k # \<Gamma>" by (simp add: fresh_Cons)
-  obtain \<tau>2 where P: "BVar x \<tau>1 # BTyVar a k # \<Gamma> \<turnstile> e : \<tau>2" "\<sigma> = (\<tau>1 \<rightarrow> \<tau>2)" "BTyVar a k # \<Gamma> \<turnstile>\<^sub>t\<^sub>y \<tau>1 : \<star>" using T_Abs_Inv[OF Lam(8) 1] by blast
-  then have 2: "BTyVar a k # BVar x \<tau>1 # \<Gamma> \<turnstile> e : \<tau>2" using context_invariance[OF P(1)] by simp
-  have 3: "BTyVar a k # \<Gamma>' \<turnstile>\<^sub>t\<^sub>y \<tau>1 : \<star>" using context_invariance_ty[OF P(3)] by (smt Lam.prems(3) isin.simps(5))
-  have 4: "\<Gamma>' \<turnstile>\<^sub>t\<^sub>y \<tau>' : k" using context_invariance_ty[OF Lam(9)] Lam.prems(3) by blast
-  have 5: "\<Gamma>' \<turnstile>\<^sub>t\<^sub>y subst_type \<tau>' a \<tau>1 : \<star>" using "3" "4" Lam.prems(5) type_substitution_ty by blast
-  have 6: "BVar x \<tau>1 # \<Gamma> \<turnstile>\<^sub>t\<^sub>y \<tau>' : k" using context_invariance_ty[OF Lam(9)] by auto
-
-  from 4 have 7: "atom a \<sharp> \<tau>'" using Lam.prems(5) ty_fresh_vars by blast
-  have 8: "atom a \<sharp> BVar x (subst_type \<tau>' a \<tau>1) # \<Gamma>'" using "5" Lam.prems(5) fresh_Cons ty_fresh_vars by fastforce
-
-  have 9: "BVar x (subst_type \<tau>' a \<tau>1) # \<Gamma>' \<turnstile> subst_term_type \<tau>' a e : subst_type \<tau>' a \<tau>2" using Lam(7)[OF 2 6 _ _ 8] by (simp add: Lam.prems(3) Lam.prems(4))
-
-  have "\<Gamma>' \<turnstile> \<lambda>x : subst_type \<tau>' a \<tau>1 . subst_term_type \<tau>' a e : subst_type \<tau>' a \<tau>1 \<rightarrow> subst_type \<tau>' a \<tau>2" by (rule T.T_AbsI[OF Lam(4) 5 9])
-  then show ?case using P(2) by simp
+  have 1: "atom x \<sharp> \<Gamma> @ \<Gamma>'" using fresh_append Lam(1,2) by blast
+  obtain \<tau>2 where P: "(BVar x \<tau>1 # \<Gamma>) @ \<Gamma>' \<turnstile> e : \<tau>2" "\<tau> = (\<tau>1 \<rightarrow> \<tau>2)" using T_Abs_Inv[OF Lam(6) 1] by auto
+  have 2: "\<Gamma> @ \<Gamma>' \<turnstile>\<^sub>t\<^sub>y \<tau>1 : \<star>" by (cases rule: Ctx.cases[OF tm_context_valid[OF P(1)]]) auto
+  have 3: "\<Gamma> @ xs @ \<Gamma>' \<turnstile>\<^sub>t\<^sub>y \<tau>1 : \<star>" by (rule weaken_ty[OF 2 Lam(7)])
+  have 4: "atom x \<sharp> \<Gamma> @ xs @ \<Gamma>'" using fresh_append Lam(1-3) by blast
+  have 5: "\<turnstile> (BVar x \<tau>1 # \<Gamma>) @ xs @ \<Gamma>'" using Ctx_Var[OF 3 4] by simp
+  have 6: "BVar x \<tau>1 # \<Gamma> @ xs @ \<Gamma>' \<turnstile> e : \<tau>2" using Lam(5)[OF P(1) 5] by simp
+  show ?case using Tm_Abs[OF 6] P(2) by simp
 next
-  case (TyLam b k2 e)
-  then have 1: "atom b \<sharp> BTyVar a k # \<Gamma>" by (simp add: fresh_Cons)
-  obtain \<tau> where P: "BTyVar b k2 # BTyVar a k # \<Gamma> \<turnstile> e : \<tau>" "\<sigma> = (\<forall> b : k2 . \<tau>)" using T_AbsT_Inv[OF TyLam(8) 1 TyLam(5)] by blast
-  then have 2: "subst_type \<tau>' a \<sigma> = (\<forall> b : k2 . subst_type \<tau>' a \<tau>)" by (simp add: TyLam(1) TyLam(6))
-  have 3: "BTyVar a k # BTyVar b k2 # \<Gamma> \<turnstile> e : \<tau>" using context_invariance[OF P(1)] by (smt TyLam.hyps(1) fresh_at_base(2) isin.simps(3) isin.simps(5))
-  have 4: "BTyVar b k2 # \<Gamma> \<turnstile>\<^sub>t\<^sub>y \<tau>' : k" using context_invariance_ty[OF TyLam(9)] by (simp add: TyLam.hyps(3) fresh_not_isin_tyvar)
-  have 5: "atom a \<sharp> BTyVar b k2 # \<Gamma>'" using TyLam(1) TyLam.prems(5) fresh_Cons by fastforce
-
-  have 9: "BTyVar b k2 # \<Gamma>' \<turnstile> subst_term_type \<tau>' a e : subst_type \<tau>' a \<tau>" using TyLam(7)[OF 3 4 _ _ 5] TyLam(10) TyLam(11) by simp
-
-  show ?case using T.T_AbsTI[OF 9 TyLam(4)] 2 TyLam(1) TyLam(6) by simp
+  case (TyLam a k e)
+  have 1: "atom a \<sharp> \<Gamma> @ \<Gamma>'" using fresh_append TyLam(1,2) by blast
+  obtain \<sigma> where P: "(BTyVar a k # \<Gamma>) @ \<Gamma>' \<turnstile> e : \<sigma>" "\<tau> = (\<forall> a : k . \<sigma>)" using T_AbsT_Inv[OF TyLam(6) 1 TyLam(4)] by auto
+  have 2: "atom a \<sharp> \<Gamma> @ xs @ \<Gamma>'" using fresh_append TyLam(1-3) by blast
+  have 3: "\<turnstile> (BTyVar a k # \<Gamma>) @ xs @ \<Gamma>'" using Ctx_TyVar[OF TyLam(7) 2] by simp
+  have 4: "BTyVar a k # \<Gamma> @ xs @ \<Gamma>' \<turnstile> e : \<sigma>" using TyLam(5)[OF P(1) 3] by simp
+  show ?case using Tm_TAbs[OF 4] P(2) by simp
 next
   case (Let x \<tau>1 e1 e2)
-  then have 1: "atom x \<sharp> BTyVar a k # \<Gamma>" by (simp add: fresh_Cons)
-  have P: "BTyVar a k # \<Gamma> \<turnstile> e1 : \<tau>1" "BVar x \<tau>1 # BTyVar a k # \<Gamma> \<turnstile> e2 : \<sigma>" using T_Let_Inv[OF Let(9) 1] by auto
-  have 2: "atom x \<sharp> e1" using "1" P(1) fresh_term_var by blast
-  have "atom x \<sharp> subst_term_type \<tau>' a e1" using Let P(1) fresh_term_var by blast
-  then have 3: "atom x \<sharp> (\<Gamma>', subst_term_type \<tau>' a e1)" using Let(4) by simp
-  have 5: "atom a \<sharp> BVar x (subst_type \<tau>' a \<tau>1) # \<Gamma>'"
-    by (metis Let.hyps(1) Let.prems(2) Let.prems(3) Let.prems(5) binder.fresh(1) context_invariance_ty fresh_Cons fresh_at_base(2) fresh_subst_type ty_fresh_vars)
-  have 6: "BTyVar a k # BVar x \<tau>1 # \<Gamma> \<turnstile> e2 : \<sigma>" using context_invariance[OF P(2)] by auto
-  have 7: "BVar x \<tau>1 # \<Gamma> \<turnstile>\<^sub>t\<^sub>y \<tau>' : k" using Let.prems(2) context_invariance_ty isin.simps(4) by blast
-
-  have 9: "BVar x (subst_type \<tau>' a \<tau>1) # \<Gamma>' \<turnstile> subst_term_type \<tau>' a e2 : subst_type \<tau>' a \<sigma>" using Let(8)[OF 6 7 _ _ 5] Let(11) Let(12) by simp
-  show ?case using T.T_LetI[OF 3 9] using Let P(1) by auto
+  have 1: "atom x \<sharp> \<Gamma> @ \<Gamma>'" using fresh_append Let(1,2) by blast
+  have P: "\<Gamma> @ \<Gamma>' \<turnstile> e1 : \<tau>1" "(BVar x \<tau>1 # \<Gamma>) @ \<Gamma>' \<turnstile> e2 : \<tau>" using T_Let_Inv[OF Let(7) 1] by auto
+  have 2: "\<Gamma> @ xs @ \<Gamma>' \<turnstile> e1 : \<tau>1" by (rule Let(5)[OF P(1) Let(8)])
+  have 3: "\<Gamma> @ \<Gamma>' \<turnstile>\<^sub>t\<^sub>y \<tau>1 : \<star>" by (cases rule: Ctx.cases[OF tm_context_valid[OF P(2)]]) auto
+  have 4: "\<Gamma> @ xs @ \<Gamma>' \<turnstile>\<^sub>t\<^sub>y \<tau>1 : \<star>" by (rule weaken_ty[OF 3 Let(8)])
+  have 5: "atom x \<sharp> \<Gamma> @ xs @ \<Gamma>'" using fresh_append Let(1-3) by blast
+  have 6: "\<turnstile> (BVar x \<tau>1 # \<Gamma>) @ xs @ \<Gamma>'" using Ctx_Var[OF 4 5] by simp
+  have 7: "BVar x \<tau>1 # \<Gamma> @ xs @ \<Gamma>' \<turnstile> e2 : \<tau>" using Let(6)[OF P(2) 6] by simp
+  show ?case by (rule Tm_Let[OF 2 7])
 qed
 
-theorem preservation: "\<lbrakk> [] \<turnstile> e : \<tau> ; e \<longrightarrow> e' \<rbrakk> \<Longrightarrow> [] \<turnstile> e' : \<tau>"
-proof (nominal_induct "[] :: \<Gamma>" e \<tau> arbitrary: e' rule: T.strong_induct)
-  case T_UnitI
-  then show ?case using Step.cases by fastforce
+lemma type_substitution_aux:
+  assumes "\<Gamma> \<turnstile>\<^sub>t\<^sub>y \<sigma> : k"
+  shows "(\<turnstile> (\<Gamma>' @ BTyVar a k # \<Gamma>) \<longrightarrow> \<turnstile> (subst_context \<Gamma>' \<sigma> a @ \<Gamma>)) \<and> ((\<Gamma>' @ BTyVar a k # \<Gamma>) \<turnstile>\<^sub>t\<^sub>y \<tau> : k2 \<longrightarrow> (subst_context \<Gamma>' \<sigma> a @ \<Gamma>) \<turnstile>\<^sub>t\<^sub>y subst_type \<tau> \<sigma> a : k2)"
+proof (rule Ctx_Ty_induct)
+  show "\<turnstile> [][\<sigma>/a] @ \<Gamma>" using ty_context_valid[OF assms(1)] by simp
 next
-  case (T_VarI x \<tau>)
-  then show ?case by simp
+  fix \<Gamma>' a2 k2
+  assume a: "\<turnstile> \<Gamma>' @ BTyVar a k # \<Gamma>" "\<turnstile> \<Gamma>'[\<sigma>/a] @ \<Gamma>" "atom (a2::tyvar) \<sharp> \<Gamma>' @ BTyVar a k # \<Gamma>"
+  then have "atom a2 \<sharp> \<sigma>" using assms fresh_in_context(2) fresh_Cons fresh_append by blast 
+  then have 1: "atom a2 \<sharp> \<Gamma>'[\<sigma>/a] @ \<Gamma>" by (meson a(3) fresh_Cons fresh_append fresh_subst_context_tyvar)
+  show "\<turnstile> (BTyVar a2 k2 # \<Gamma>')[\<sigma>/a] @ \<Gamma>" using Ctx_TyVar[OF a(2) 1] assms by auto
 next
-  case (T_AbsI x \<tau>1 e \<tau>2)
-  then show ?case using Step.cases by fastforce
+  fix \<Gamma>' \<tau> x
+  assume a: "\<Gamma>' @ BTyVar a k # \<Gamma> \<turnstile>\<^sub>t\<^sub>y \<tau> : \<star>" "\<Gamma>'[\<sigma>/a] @ \<Gamma> \<turnstile>\<^sub>t\<^sub>y \<tau>[\<sigma>/a] : \<star>" "atom (x::var) \<sharp> \<Gamma>' @ BTyVar a k # \<Gamma>"
+  have 1: "atom x \<sharp> \<Gamma>'[\<sigma>/a] @ \<Gamma>" by (meson a(3) fresh_Cons fresh_append fresh_subst_context_var)
+  show "\<turnstile> (BVar x \<tau> # \<Gamma>')[\<sigma>/a] @ \<Gamma>" using Ctx_Var[OF a(2) 1] by simp
 next
-  case (T_AppI e1 \<tau>1 \<tau>2 e2)
-  from \<open>App e1 e2 \<longrightarrow> e'\<close> show ?case
-  proof cases
-    case (ST_BetaI x \<tau> e)
-    then have "\<tau> = \<tau>1" using T_AppI.hyps(1) fun_ty_lam is_value.simps(2) term.eq_iff(5) by blast
-    then have 1: "[] \<turnstile> e2 : \<tau>" using T_AppI(3) by simp
-
-    have "[] \<turnstile> \<lambda> x : \<tau> . e : \<tau>1 \<rightarrow> \<tau>2" using T_AppI ST_BetaI by blast
-    then have 2: "[BVar x \<tau>] \<turnstile> e : \<tau>2" using T_Abs_Inv fresh_Nil by fastforce
-
-    show ?thesis using substitution[OF 2 1] ST_BetaI by simp
+  fix \<Gamma>' a2 k2
+  assume a: "\<turnstile> \<Gamma>' @ BTyVar a k # \<Gamma>" "\<turnstile> \<Gamma>'[\<sigma>/a] @ \<Gamma>" "BTyVar a2 k2 \<in> (\<Gamma>' @ BTyVar a k # \<Gamma>)"
+  then show "\<Gamma>'[\<sigma>/a] @ \<Gamma> \<turnstile>\<^sub>t\<^sub>y (TyVar a2)[\<sigma>/a] : k2"
+  proof (cases "a2 = a")
+    case True
+    then have "k = k2" using isin_kind_same a by blast
+    then have "\<Gamma> \<turnstile>\<^sub>t\<^sub>y (TyVar a2)[\<sigma>/a] : k2" using True assms(1) by simp
+    then show ?thesis using weaken_ty[of "[]"] a(2) by auto
   next
-    case (ST_AppI e2)
-    then show ?thesis using T_AppI T.T_AppI by blast
+    case False
+    have 1: "BTyVar a2 k2 \<in> (\<Gamma>'[\<sigma>/a] @ \<Gamma>)" by (rule isin_subst[OF a(3,1) False])
+    show ?thesis using Ty_Var[OF a(2) 1] False by simp
   qed
 next
-  case (T_LetI x e1 \<tau>1 e2 \<tau>2)
-  from \<open>Let x \<tau>1 e1 e2 \<longrightarrow> e'\<close> show ?case
-  proof cases
-    case (ST_SubstI y e)
-    then show ?thesis
-    proof (cases "atom x = atom y")
-      case True
-      then show ?thesis by (metis Abs1_eq(3) T_LetI.hyps(3) T_LetI.hyps(4) atom_eq_iff local.ST_SubstI(1) local.ST_SubstI(2) substitution)
-    next
-      case False
-      then have 1: "atom y \<sharp> [(x, \<tau>1)]" by (simp add: fresh_Cons fresh_Nil)
-      have "(x \<leftrightarrow> y) \<bullet> e2 = e" by (metis Abs1_eq_iff'(3) False flip_commute local.ST_SubstI(1))
-      then have "[BVar y \<tau>1] \<turnstile> e : \<tau>2" using T.eqvt
-        by (metis Cons_eqvt Nil_eqvt T_LetI.hyps(3) binder.perm_simps(1) flip_at_simps(1) flip_fresh_fresh no_vars_in_ty)
-      then show ?thesis using T_LetI ST_SubstI substitution by auto
-    qed
-  qed
-next
-  case (T_AppTI e a k \<sigma> \<tau>)
-  from T_AppTI(4) show ?case
-  proof cases
-    case (ST_BetaTI b k2 t)
-    obtain c::tyvar where "atom c \<sharp> (a, b, t, \<sigma>)" using obtain_fresh by blast
-    then have c: "atom c \<sharp> a" "atom c \<sharp> b" "atom c \<sharp> t" "atom c \<sharp> \<sigma>" using fresh_Pair by auto
-    have 1: "[] \<turnstile> (\<Lambda> c : k2 . (b \<leftrightarrow> c) \<bullet> t) : \<forall> c : k2 . (a \<leftrightarrow> c) \<bullet> \<sigma>"
-      by (smt Abs1_eq_iff(3) T.cases T_AppTI.hyps(1) \<tau>.distinct(17) \<tau>.distinct(7) \<tau>.eq_iff(5) c(1) c(2) c(3) c(4) flip_commute fresh_at_base(2) is_value.simps(3) is_value.simps(4) is_value.simps(5) is_value.simps(7) isin.simps(1) local.ST_BetaTI(1) term.eq_iff(6))
+  fix b k2 \<Gamma>' \<sigma>'
+  assume a: "(BTyVar b k2 # \<Gamma>' @ BTyVar a k # \<Gamma>) \<turnstile>\<^sub>t\<^sub>y \<sigma>' : \<star>" "(BTyVar b k2 # \<Gamma>')[\<sigma>/a] @ \<Gamma> \<turnstile>\<^sub>t\<^sub>y \<sigma>'[\<sigma>/a] : \<star>"
+  have 1: "a \<noteq> b" by (metis a(1) binder.fresh(2) context_cons_fresh_tyvar fresh_Cons fresh_append fresh_at_base(2) ty_context_valid)
+  then have 2: "BTyVar b k2 # \<Gamma>'[\<sigma>/a] @ \<Gamma> \<turnstile>\<^sub>t\<^sub>y \<sigma>'[\<sigma>/a] : \<star>" using a(2) by simp
+  show "\<Gamma>'[\<sigma>/a] @ \<Gamma> \<turnstile>\<^sub>t\<^sub>y (\<forall> b : k2 . \<sigma>')[\<sigma>/a] : \<star>" using Ty_Forall[OF 2]
+    by (metis "1" "2" assms atom_eq_iff context_cons_fresh_tyvar fresh_Pair fresh_append fresh_at_base(2) subst_type.simps(5) ty_context_valid ty_fresh_vars)
+qed (auto intro: Ty_intros)
 
-    have 2: "[BTyVar c k2] \<turnstile> (b \<leftrightarrow> c) \<bullet> t : (a \<leftrightarrow> c) \<bullet> \<sigma>"
-    proof (cases rule: T.cases[OF 1])
-      case (7 a' k2' \<Gamma> e \<sigma>')
-      then have same: "k2 = k2'" using \<tau>.eq_iff(5) by blast
-      have 1: "(b \<leftrightarrow> c) \<bullet> t = (a' \<leftrightarrow> c) \<bullet> e"
-        by (metis (no_types, lifting) "7"(2) Abs1_eq_iff(3) Nominal2_Base.swap_self add_flip_cancel flip_commute flip_def permute_flip_cancel2 permute_plus term.eq_iff(6))
-      have 2: "(a \<leftrightarrow> c) \<bullet> \<sigma> = (a' \<leftrightarrow> c) \<bullet> \<sigma>'"
-        by (metis "7"(3) Abs1_eq_iff(3) Nominal2_Base.swap_self \<tau>.eq_iff(5) c(4) flip_commute flip_def swap_fresh_fresh)
-      from 7(4) have 3: "(a' \<leftrightarrow> c) \<bullet> (BTyVar a' k2' # \<Gamma> \<turnstile> e : \<sigma>')" by simp
-      have 4: "(a' \<leftrightarrow> c) \<bullet> (BTyVar a' k2' # \<Gamma>) = ((a' \<leftrightarrow> c) \<bullet> BTyVar a' k2') # \<Gamma>" using "7"(1) by auto
-      have 5: "(a' \<leftrightarrow> c) \<bullet> BTyVar a' k2' = BTyVar c k2'" using flip_fresh_fresh[OF no_tyvars_in_kinds[of a' k2'] no_tyvars_in_kinds[of c k2']] flip_at_base_simps(1)[of a' c] by simp
-
-      show ?thesis using T.eqvt[OF 7(4), of "(a' \<leftrightarrow> c)"] using "1" "2" "5" "7"(1) same by auto
-    qed auto
-    have "k = k2" using T.cases T_AppTI.hyps(1) local.ST_BetaTI(1) by fastforce
-    then have "[] \<turnstile> subst_term_type \<tau> c ((b \<leftrightarrow> c) \<bullet> t) : subst_type \<tau> c ((a \<leftrightarrow> c) \<bullet> \<sigma>)" using type_substitution[OF 2 _ _ _ fresh_Nil] T_AppTI(3) by simp
-    then show ?thesis using ST_BetaTI(2) subst_term_type_var_name[OF c(3)] subst_type_var_name[OF c(4)] by presburger
-  next
-    case (ST_AppTI e2)
-    then show ?thesis using T.T_AppTI T_AppTI.hyps(2) T_AppTI.hyps(3) by blast
-  qed
-next
-  case (T_AbsTI a e \<sigma>)
-  then show ?case using beta_nf_def is_value.simps(3) value_beta_nf by blast
-qed
-
-lemma multi_preservation: "\<lbrakk> e \<longrightarrow>* e' ; [] \<turnstile> e : \<tau> \<rbrakk> \<Longrightarrow> [] \<turnstile> e' : \<tau>"
-  by (induction e e' rule: Steps.induct) (auto simp: preservation)
-
-corollary soundness: "\<lbrakk> [] \<turnstile> e : \<tau> ; e \<longrightarrow>* e' \<rbrakk> \<Longrightarrow> \<not>(stuck e')"
-  unfolding stuck_def beta_nf_def
-  using progress multi_preservation by blast
+corollary type_substitution_context: "\<lbrakk> \<turnstile> \<Gamma>' @ BTyVar a k # \<Gamma> ; \<Gamma> \<turnstile>\<^sub>t\<^sub>y \<sigma> : k \<rbrakk> \<Longrightarrow> \<turnstile> \<Gamma>'[\<sigma>/a] @ \<Gamma>"
+  using type_substitution_aux by blast
+corollary type_substitution_ty: "\<lbrakk> \<Gamma>' @ BTyVar a k # \<Gamma> \<turnstile>\<^sub>t\<^sub>y \<tau> : k2 ; \<Gamma> \<turnstile>\<^sub>t\<^sub>y \<sigma> : k \<rbrakk> \<Longrightarrow> \<Gamma>'[\<sigma>/a] @ \<Gamma> \<turnstile>\<^sub>t\<^sub>y \<tau>[\<sigma>/a] : k2"
+  using type_substitution_aux by blast
 
 end
